Split stateis.v off from rest of spred

src/spred/core.v
@@ -504,80 +504,6 @@ Local Opaque SABIOps.
 
 Global Coercion lbool (b:bool) := lpropand b ltrue.
 
-(*===========================================================================
-    "is" predicates on registers and flags
-  ===========================================================================*)
-
-Definition regPieceIs r v : SPred := eq_pred (addRegPieceToPState emptyPState r v).
-Definition flagIs f b : SPred := eq_pred (addFlagToPState emptyPState f b).
-(*Definition BYTEregIs (r:Reg OpSize1) v : SPred := regPieceIs (BYTERegToRegPiece r) v.*)
-
-Definition reg64Is (r:Reg64) (v:QWORD) : SPred :=
-  let pi i := regPieceIs (mkRegPiece r i) (getRegPiece v i) in
-   pi 0 ** pi 1 ** pi 2 ** pi 3 ** pi 4 ** pi 5 ** pi 6 ** pi 7.
-
-Definition reg32Is (r:Reg32) (v:DWORD) : SPred :=
-  let pi i := regPieceIs (mkRegPiece (Reg32_base r) i) (getRegPiece v i) in
-   pi 0 ** pi 1 ** pi 2 ** pi 3.
-
-Definition reg16Is (r:Reg16) (v:WORD) : SPred :=
-   regPieceIs (mkRegPiece (Reg16_base r) 0) (slice 0 8 8 v)
-** regPieceIs (mkRegPiece (Reg16_base r) 1) (slice 8 8 0 v).
-
-Definition reg8Is (r:Reg8) (v:BYTE) : SPred :=
-   regPieceIs (mkRegPiece (Reg8_base r) 0) v.
-
-Inductive RegOrFlag :=
-| RegOrFlagR s :> Reg s -> RegOrFlag
-| RegOrFlagF :> Flag -> RegOrFlag.
-
-Definition RegOrFlag_target rf :=
-match rf with
-| RegOrFlagR s _   => VWORD s
-| RegOrFlagF _     => FlagVal
-end.
-
-Definition stateIs (x: RegOrFlag) : RegOrFlag_target x -> SPred :=
-match x with
-| RegOrFlagR OpSize1 r => reg8Is r
-| RegOrFlagR OpSize2 r => reg16Is r
-| RegOrFlagR OpSize4 r => reg32Is r
-| RegOrFlagR OpSize8 r => reg64Is r
-| RegOrFlagF f => flagIs f
-end.
-
-Implicit Arguments stateIs [].
-
-Definition stateIsAny x := lexists (stateIs x).
-
-Notation "x '~=' v" := (stateIs x v) (at level 70, no associativity, format "x '~=' v") : spred_scope.
-Notation "x '?'" := (stateIsAny x) (at level 2, format "x '?'"): spred_scope.
-
-Hint Unfold VWORD RegOrFlag_target : spred.
-(** When dealing with logic, we want to reduce [stateIsAny] and similar to basic building blocks. *)
-Hint Unfold stateIsAny : finish_logic_unfolder.
-
-(*---------------------------------------------------------------------------
-     Byte-is predicate
-  ---------------------------------------------------------------------------*)
-Program Definition byteIs p b : SPred := eq_pred (addBYTEToPState emptyPState p b).
-
-Definition byteAny p : SPred := lexists (byteIs p).
-
-Instance flagIsEquiv_m :
-  Proper (eq ==> eq ==> csetoid.equiv ==> iff) flagIs.
-Proof.
-  intros n m Hneqm f g Hbeqc p q Hpeqq; subst.
-  split; simpl; rewrite <- Hpeqq; tauto.
-Qed.
-
-Instance byteIsEquiv_m :
-  Proper (eq ==> eq ==> csetoid.equiv ==> iff) byteIs.
-Proof.
-  intros n m Hneqm b c Hbeqc p q Hpeqq; subst.
-  split; simpl; rewrite <- Hpeqq; tauto.
-Qed.
-
 (*---------------------------------------------------------------------------
     Iterated separating conjunction
   ---------------------------------------------------------------------------*)
@@ -610,15 +536,6 @@ Proof. rewrite isc_cat /=. by rewrite empSPR. Qed.
 Class StrictlyExact (P: SPred) := strictly_exact:
   forall s s', P s -> P s' -> s === s'.
 
-Instance StrictlyExactRegPieceIs r v: StrictlyExact (regPieceIs r v).
-Proof. move => s s'. simpl. by move ->. Qed.
-
-Instance StrictlyExactFlagIs f v: StrictlyExact (flagIs f v).
-Proof. move => s s'. simpl. by move ->. Qed.
-
-Instance StrictlyExactByteIs p v: StrictlyExact (byteIs p v).
-Proof. move => s s'. simpl. by move ->. Qed.
-
 Instance StrictlyExactSep P Q `{PH: StrictlyExact P} `{QH: StrictlyExact Q}
   : StrictlyExact (P**Q).
 Proof. move => s s' [s1 [s2 [H1 [H2 H3]]]] [s1' [s2' [H1' [H2' H3']]]].
@@ -627,10 +544,6 @@ specialize (QH s2 s2' H3 H3').
 rewrite -> PH, QH in H1.
 by rewrite (stateSplitsAsExtends H1) (stateSplitsAsExtends H1').
 Qed.
-
-Instance StrictlyExactRegIs r v: StrictlyExact (reg64Is r v).
-Proof. rewrite /reg64Is. do 7 (apply StrictlyExactSep; first apply StrictlyExactRegPieceIs).
-apply StrictlyExactRegPieceIs. Qed.
 
 Instance StrictlyExactEmpSP : StrictlyExact empSP.
 Proof. move => s s' H H'.
@@ -703,46 +616,25 @@ Qed.
 Global Opaque PStateSepAlgOps.
 
 (*---------------------------------------------------------------------------
+     Byte-is predicate
+  ---------------------------------------------------------------------------*)
+Program Definition byteIs p b : SPred := eq_pred (addBYTEToPState emptyPState p b).
+
+Definition byteAny p : SPred := lexists (byteIs p).
+
+Instance byteIsEquiv_m :
+  Proper (eq ==> eq ==> csetoid.equiv ==> iff) byteIs.
+Proof.
+  intros n m Hneqm b c Hbeqc p q Hpeqq; subst.
+  split; simpl; rewrite <- Hpeqq; tauto.
+Qed.
+
+Instance StrictlyExactByteIs p v: StrictlyExact (byteIs p v).
+Proof. move => s s'. simpl. by move ->. Qed.
+
+(*---------------------------------------------------------------------------
     Some lemmas about the domains of primitive points-to-like predicates
   ---------------------------------------------------------------------------*)
-Open Scope spred_scope.
-
-Lemma regPieceIs_same (r:RegPiece) v1 v2 : regPieceIs r v1 ** regPieceIs r v2 |-- lfalse.
-Proof.  move => s [s1 [s2 [H1 [H1a H1b]]]].
-simpl in H1a, H1b. rewrite <-H1a in H1. rewrite <-H1b in H1.
-rewrite /sa_mul/PStateSepAlgOps/= in H1.
-specialize (H1 Registers r). simpl in H1.
-destruct (s Registers r); rewrite eq_refl in H1.
-destruct H1; by destruct H.
-by destruct H1.
-Qed.
-
-Lemma sepRev4 P Q R S : P ** Q ** R ** S -|- S ** R ** Q ** P.
-Proof. rewrite (sepSPC P). rewrite (sepSPC Q). rewrite (sepSPC R).
-by rewrite !sepSPA. Qed.
-
-(*
-Lemma regIs_same s (r:VRegAny s) (v1 v2:VWORD s) : r ~= v1 ** r ~= v2 |-- lfalse.
-Proof. destruct s. 
-- apply regPieceIs_same. 
-- destruct r. admit. 
-- rewrite /stateIs/regIs. 
-  rewrite sepRev4. rewrite sepSPA.
-  rewrite sepRev4. rewrite -!sepSPA. rewrite -> (@regPieceIs_same (AnyRegPiece r (inord 0))).
-  by rewrite !sepSP_falseL. 
-Qed.
-*)
-
-Lemma flagIs_same (f:Flag) v1 v2 : f ~= v1 ** f ~= v2 |-- lfalse.
-Proof.  move => s [s1 [s2 [H1 [H1a H1b]]]].
-simpl in H1a, H1b. rewrite <-H1a in H1. rewrite <-H1b in H1.
-rewrite /sa_mul/PStateSepAlgOps/= in H1.
-specialize (H1 Flags f). simpl in H1.
-destruct (s Flags f); rewrite eq_refl in H1.
-destruct H1; by destruct H.
-by destruct H1.
-Qed.
-
 Lemma byteIs_same p v1 v2 : byteIs p v1 ** byteIs p v2 |-- lfalse.
 Proof.  move => s [s1 [s2 [H1 [H1a H1b]]]].
 simpl in H1a, H1b. rewrite <-H1a in H1. rewrite <-H1b in H1.
@@ -752,7 +644,4 @@ destruct (s Memory p); rewrite eq_refl in H1.
 destruct H1; by destruct H.
 by destruct H1.
 Qed.
-
-(* We don't want simpl to unfold this *)
-Global Opaque stateIs.
 
