src/spred.v
@@ -1,6 +1,7 @@
 (** * Predicates over partial states *)
 
 Require Export x86proved.spred.core.
-Require Export x86proved.spred.septac.
+Require Export x86proved.spred.stateis.
+Require Export x86proved.spred.tactics.
 (* Important: the ssimpl tactic in pointsto overrides the one in septac *)
 Require Export x86proved.spred.pointsto.
