src/spred/stateis.v
@@ -1,0 +1,154 @@
+(*===========================================================================
+    stateIs predicate for registers and flags
+  ===========================================================================*)
+Require Import Ssreflect.ssreflect Ssreflect.ssrfun Ssreflect.ssrbool Ssreflect.eqtype Ssreflect.fintype Ssreflect.finfun Ssreflect.seq Ssreflect.tuple.
+Require Import x86proved.bitsrep x86proved.pfun x86proved.x86.reg x86proved.x86.mem x86proved.x86.flags.
+Require Import x86proved.pmap x86proved.pmapprops x86proved.x86.addr x86proved.spred.core x86proved.spred.tactics.
+Require Import Coq.Setoids.Setoid x86proved.charge.csetoid Coq.Classes.Morphisms.
+
+Set Implicit Arguments.
+Unset Strict Implicit.
+Import Prenex Implicits.
+
+Require Import Coq.Logic.FunctionalExtensionality.
+
+Local Opaque SABIOps.
+
+Global Coercion lbool (b:bool) := lpropand b ltrue.
+
+(*===========================================================================
+    "is" predicates on registers and flags
+  ===========================================================================*)
+
+Definition regPieceIs r v : SPred := eq_pred (addRegPieceToPState emptyPState r v).
+Definition flagIs f b : SPred := eq_pred (addFlagToPState emptyPState f b).
+
+Definition reg64Is (r:Reg64) (v:QWORD) : SPred :=
+  let pi i := regPieceIs (mkRegPiece r i) (getRegPiece v i) in
+   pi 0 ** pi 1 ** pi 2 ** pi 3 ** pi 4 ** pi 5 ** pi 6 ** pi 7.
+
+Definition reg32Is (r:Reg32) (v:DWORD) : SPred :=
+  let pi i := regPieceIs (mkRegPiece (Reg32_base r) i) (getRegPiece v i) in
+   pi 0 ** pi 1 ** pi 2 ** pi 3.
+
+Definition reg16Is (r:Reg16) (v:WORD) : SPred :=
+   regPieceIs (mkRegPiece (Reg16_base r) 0) (slice 0 8 8 v)
+** regPieceIs (mkRegPiece (Reg16_base r) 1) (slice 8 8 0 v).
+
+Definition reg8Is (r:Reg8) (v:BYTE) : SPred :=
+   regPieceIs (mkRegPiece (Reg8_base r) 0) v.
+
+Inductive RegOrFlag :=
+| RegOrFlagR s :> Reg s -> RegOrFlag
+| RegOrFlagF :> Flag -> RegOrFlag.
+
+Definition RegOrFlag_target rf :=
+match rf with
+| RegOrFlagR s _   => VWORD s
+| RegOrFlagF _     => FlagVal
+end.
+
+Definition stateIs (x: RegOrFlag) : RegOrFlag_target x -> SPred :=
+match x with
+| RegOrFlagR OpSize1 r => reg8Is r
+| RegOrFlagR OpSize2 r => reg16Is r
+| RegOrFlagR OpSize4 r => reg32Is r
+| RegOrFlagR OpSize8 r => reg64Is r
+| RegOrFlagF f => flagIs f
+end.
+
+Implicit Arguments stateIs [].
+
+Definition stateIsAny x := lexists (stateIs x).
+
+Notation "x '~=' v" := (stateIs x v) (at level 70, no associativity, format "x '~=' v") : spred_scope.
+Notation "x '?'" := (stateIsAny x) (at level 2, format "x '?'"): spred_scope.
+
+Hint Unfold VWORD RegOrFlag_target : spred.
+(** When dealing with logic, we want to reduce [stateIsAny] and similar to basic building blocks. *)
+Hint Unfold stateIsAny : finish_logic_unfolder.
+
+Instance flagIsEquiv_m :
+  Proper (eq ==> eq ==> csetoid.equiv ==> iff) flagIs.
+Proof.
+  intros n m Hneqm f g Hbeqc p q Hpeqq; subst.
+  split; simpl; rewrite <- Hpeqq; tauto.
+Qed.
+
+Instance StrictlyExactRegPieceIs r v: StrictlyExact (regPieceIs r v).
+Proof. move => s s'. simpl. by move ->. Qed.
+
+Instance StrictlyExactFlagIs f v: StrictlyExact (flagIs f v).
+Proof. move => s s'. simpl. by move ->. Qed.
+
+Instance StrictlyExactByteIs p v: StrictlyExact (byteIs p v).
+Proof. move => s s'. simpl. by move ->. Qed.
+
+Instance StrictlyExactRegIs r v: StrictlyExact (reg64Is r v).
+Proof. rewrite /reg64Is. do 7 (apply StrictlyExactSep; first apply StrictlyExactRegPieceIs).
+apply StrictlyExactRegPieceIs. Qed.
+
+(*---------------------------------------------------------------------------
+    Some lemmas about the domains of primitive points-to-like predicates
+  ---------------------------------------------------------------------------*)
+Open Scope spred_scope.
+Local Transparent ILFun_Ops lentails sepILogicOps.
+
+Lemma regPieceIs_same (r:RegPiece) v1 v2 : regPieceIs r v1 ** regPieceIs r v2 |-- lfalse.
+Proof. move => s [s1 [s2 [H1 [H1a H1b]]]].
+simpl in H1a, H1b. rewrite <-H1a in H1. rewrite <-H1b in H1.
+rewrite /sa_mul/PStateSepAlgOps/= in H1.
+specialize (H1 Registers r). simpl in H1.
+destruct (s Registers r); rewrite eq_refl in H1.
+destruct H1; by destruct H.
+by destruct H1.
+Qed.
+
+Lemma sepRev4 P Q R S : P ** Q ** R ** S -|- S ** R ** Q ** P.
+Proof. rewrite (sepSPC P). rewrite (sepSPC Q). rewrite (sepSPC R).
+by rewrite !sepSPA. Qed.
+
+
+Lemma regIs_same s (r:Reg s) (v1 v2:VWORD s) : r ~= v1 ** r ~= v2 |-- lfalse.
+Proof. destruct s. 
+- apply regPieceIs_same. 
+- rewrite /stateIs/reg16Is. 
+  rewrite -(sepSPC (regPieceIs (mkRegPiece (Reg16_base r) 1) _)). 
+  rewrite sepSPA. setoid_rewrite <-sepSPA at 2. 
+  rewrite -> (@regPieceIs_same (mkRegPiece _ _)).
+  rewrite !sepSP_falseL.
+  by rewrite !sepSP_falseR.  
+- rewrite /stateIs/reg32Is. 
+  rewrite sepRev4. rewrite sepSPA.
+  rewrite sepRev4. rewrite -!sepSPA. rewrite -> (@regPieceIs_same (mkRegPiece _ 0)).
+  by rewrite !sepSP_falseL. 
+- rewrite /stateIs/reg64Is. 
+  rewrite sepRev4. rewrite sepSPA.
+  rewrite sepRev4. rewrite -!sepSPA. rewrite -> (@regPieceIs_same (mkRegPiece _ 0)).
+  by rewrite !sepSP_falseL. 
+Qed.
+
+Lemma flagIs_same (f:Flag) v1 v2 : f ~= v1 ** f ~= v2 |-- lfalse.
+Proof.  move => s [s1 [s2 [H1 [H1a H1b]]]].
+simpl in H1a, H1b. rewrite <-H1a in H1. rewrite <-H1b in H1.
+rewrite /sa_mul/PStateSepAlgOps/= in H1.
+specialize (H1 Flags f). simpl in H1.
+destruct (s Flags f); rewrite eq_refl in H1.
+destruct H1; by destruct H.
+by destruct H1.
+Qed.
+
+(* We don't want simpl to unfold this *)
+Global Opaque stateIs.
+
+(* Disjointness for registers, flags and bytes *)
+Lemma regIs_disjoint s (r1 r2: Reg s) v1 v2 : r1 ~= v1 ** r2 ~= v2 |-- r1 <> r2 /\\ (r1 ~= v1 ** r2 ~= v2).
+Proof. destruct s;
+(case E: (r1 == r2); [(rewrite (eqP E); by setoid_rewrite regIs_same at 1) | ssplit => H; [by rewrite H eq_refl in E| done]]). 
+Qed. 
+
+Lemma flagIs_disjoint (f1 f2: Flag) v1 v2 : f1 ~= v1 ** f2 ~= v2 |-- f1 <> f2 /\\ (f1 ~= v1 ** f2 ~= v2).
+Proof. case E: (f1 == f2). rewrite (eqP E). by setoid_rewrite flagIs_same at 1.
+ssplit; last done. move => H. by rewrite H eq_refl in E.
+Qed.
+
